add wp_nval

src/program_logic/recovery_adequacy.v
@@ -22,58 +22,43 @@ Implicit Types e : expr Λ.
 
 Notation wptp s t := ([∗ list] ef ∈ t, WPC ef @ s; ⊤ {{ fork_post }} {{ True }})%I.
 
-Notation steps_sum := crash_adequacy.steps_sum.
-
-Fixpoint step_fupdN_fresh ncurrent (ns: list nat) (HG0: generationGS Λ Σ)
+Fixpoint step_fupdN_fresh (ns: list nat) (HG0: generationGS Λ Σ)
          (P: generationGS Λ Σ → iProp Σ) {struct ns} :=
   match ns with
   | [] => P HG0
   | (n :: ns) =>
-    (£ (steps_sum (num_laters_per_step) (step_count_next) ncurrent (S n)) -∗
-      ||={⊤|⊤,∅|∅}=> ||▷=>^(steps_sum (num_laters_per_step) (step_count_next)
-                                     ncurrent (S n)) ||={∅|∅, ⊤|⊤}=>
-     ||={⊤|⊤,∅|∅}=> ||▷=>^2 ||={∅|∅, ⊤|⊤}=>
-     |={⊤}=> ∃ HG' : generationGS Λ Σ,
-       step_fupdN_fresh ((Nat.iter (S n) step_count_next ncurrent)) ns HG' P)
+      |={⊤|⊤}⧗=>^(S n)
+      ∃ HG' : generationGS Λ Σ,
+       step_fupdN_fresh ns HG' P
   end%I.
 
-Lemma step_fupdN_fresh_wand ncurr1 ncurr2 (ns: list nat) HG0 Q Q':
-  ncurr1 = ncurr2 →
-  step_fupdN_fresh ncurr1 (ns) HG0 Q -∗ (∀ HG, Q HG -∗ Q' HG)
-  -∗ step_fupdN_fresh ncurr2 ns HG0 Q'.
+Lemma step_fupdN_fresh_wand (ns: list nat) HG0 Q Q':
+  step_fupdN_fresh ns HG0 Q -∗ (∀ HG, Q HG -∗ Q' HG)
+  -∗ step_fupdN_fresh ns HG0 Q'.
 Proof.
-  revert HG0 ncurr1 ncurr2.
-  induction ns => ??? Hncurr.
+  revert HG0.
+  induction ns => ?.
   - iIntros "H Hwand". iApply "Hwand". eauto.
-  - iIntros "H Hwand Hlc". rewrite /step_fupdN_fresh -/step_fupdN_fresh.
-    rewrite {1}Hncurr.
-    iSpecialize ("H" with "Hlc").
-    iApply (step_fupd2N_inner_wand with "H"); try auto.
-    { subst. auto. }
-    iIntros "H".
-    iMod "H". iModIntro. iApply (step_fupd2N_wand with "H"). iIntros "H".
-    iMod "H". iModIntro.
-    iMod "H" as (HG') "H".
-    iExists _. iModIntro. iApply (IHns with "H").
-    { subst. auto. }
-    eauto.
+  - iIntros "H Hwand". rewrite /step_fupdN_fresh -/step_fupdN_fresh.
+    iApply (physical_stepN_wand with "H").
+    iDestruct 1 as (Hg') "H".
+    iExists _. by iApply (IHns with "H").
 Qed.
 
-Lemma wptp_recv_strong_normal_adequacy {CS Φ Φinv Φr κs' s HG} n ncurr mj D r1 e1 t1 κs t2 σ1 g1 σ2 g2 :
+Lemma wptp_recv_strong_normal_adequacy {CS Φ Φinv Φr κs' s HG} n mj D r1 e1 t1 κs t2 σ1 g1 σ2 g2 :
   nrsteps (CS := CS) r1 [n] (e1 :: t1, (σ1,g1)) κs (t2, (σ2,g2)) Normal →
   state_interp σ1 (length t1) -∗
-  global_state_interp g1 ncurr mj D (κs ++ κs') -∗
+  global_state_interp g1 mj D (κs ++ κs') -∗
   wpr CS s HG ⊤ e1 r1 Φ Φinv Φr -∗
   wptp s t1 -∗ NC 1-∗ (
-    (£ (steps_sum num_laters_per_step step_count_next ncurr n) -∗
-     ||={⊤|⊤,∅|∅}=> ||▷=>^(steps_sum num_laters_per_step step_count_next ncurr n) ||={∅|∅,⊤|⊤}=>
+    |={⊤|⊤}⧗=>^n ||={⊤|⊤, ⊤|⊤}=>
     ∃ e2 t2',
     ⌜ t2 = e2 :: t2' ⌝ ∗
     state_interp σ2 (length t2') ∗
-    global_state_interp g2 (Nat.iter n step_count_next ncurr) mj D κs' ∗
+    global_state_interp g2 mj D κs' ∗
     from_option Φ True (to_val e2) ∗
     ([∗ list] v ∈ omap to_val t2', fork_post v) ∗
-    NC 1)).
+    NC 1).
 Proof.
   iIntros (Hstep) "Hσ Hg He Ht HNC".
   inversion Hstep. subst.
@@ -82,22 +67,20 @@ Proof.
   {rewrite wpr_unfold /wpr_pre. iApply "He". }
   iSpecialize ("H" with "[$]").
   rewrite /step_fupdN_fresh.
-  iIntros "Hlc". iSpecialize ("H" with "Hlc").
-  iApply (step_fupd2N_wand with "H"); auto.
+  iApply (physical_stepN_wand with "H").
+  iIntros "$".
 Qed.
 
-Lemma wptp_recv_normal_progress {CS Φ Φinv Φr κs' HG} n ns ncurr mj D r1 e1 t1 κs t2 σ1 g1 σ2 g2 e2 :
+Lemma wptp_recv_normal_progress {CS Φ Φinv Φr κs' HG} n ns mj D r1 e1 t1 κs t2 σ1 g1 σ2 g2 e2 :
   nrsteps (CS := CS) r1 (ns ++ [n]) (e1 :: t1, (σ1,g1)) κs (t2, (σ2,g2)) Normal →
   e2 ∈ t2 →
   state_interp σ1 (length t1) -∗
-  global_state_interp g1 ncurr mj D (κs ++ κs') -∗
+  global_state_interp g1 mj D (κs ++ κs') -∗
   wpr CS NotStuck HG ⊤ e1 r1 Φ Φinv Φr -∗
-  wptp NotStuck t1 -∗ NC 1-∗ step_fupdN_fresh ncurr ns HG (λ HG',
+  wptp NotStuck t1 -∗ NC 1-∗ step_fupdN_fresh ns HG (λ HG',
     ⌜ HG' = HG ⌝ ∗
-  (£ (steps_sum num_laters_per_step step_count_next ncurr (S n)) -∗
-   ||={⊤|⊤,∅|∅}=> ||▷=>^(steps_sum num_laters_per_step step_count_next ncurr n) ||={∅|∅, ∅|∅}=>
-   ||▷=>^(num_laters_per_step (Nat.iter n step_count_next ncurr) + 1)
-        ⌜ not_stuck e2 σ2 g2 ⌝ )).
+    |={⊤|⊤}⧗=>^n ||={⊤|⊤, ∅|∅}=>
+        ⌜ not_stuck e2 σ2 g2 ⌝ ).
 Proof.
   iIntros (Hstep Hel) "Hσ Hg He Ht HNC".
   inversion Hstep. subst.
@@ -109,9 +92,7 @@ Proof.
     first by (eapply nrsteps_normal_empty_prefix; eauto).
   inversion H. subst.
   rewrite /step_fupdN_fresh.
-  iSplitL ""; first by eauto.
-  iIntros "Hlc". iSpecialize ("H" with "Hlc").
-  iApply (step_fupd2N_wand with "H"); auto.
+  iSplitL ""; by eauto.
 Qed.
 
 Fixpoint sum_crash_steps ns :=
@@ -120,29 +101,24 @@ Fixpoint sum_crash_steps ns :=
   | n :: ns => (S n) + (sum_crash_steps ns)
   end.
 
-Lemma wptp_recv_strong_crash_adequacy {CS Φ Φinv Φinv' Φr κs' s HG} ncurr mj D ns n r1 e1 t1 κs t2 σ1 g1 σ2 g2 :
+Lemma wptp_recv_strong_crash_adequacy {CS Φ Φinv Φinv' Φr κs' s HG} mj D ns n r1 e1 t1 κs t2 σ1 g1 σ2 g2 :
   nrsteps (CS := CS) r1 (ns ++ [n]) (e1 :: t1, (σ1,g1)) κs (t2, (σ2,g2)) Crashed →
   state_interp σ1 (length t1) -∗
-  global_state_interp g1 ncurr mj D (κs ++ κs') -∗
+  global_state_interp g1 mj D (κs ++ κs') -∗
   wpr CS s HG ⊤ e1 r1 Φ Φinv Φr -∗
   □ (∀ HG', Φinv HG' -∗ □ Φinv' HG') -∗
-  wptp s t1 -∗ NC 1-∗ step_fupdN_fresh ncurr ns HG (λ HG',
-    let ntot := (steps_sum num_laters_per_step step_count_next
-                           (Nat.iter (sum_crash_steps ns) step_count_next ncurr )
-                           n)  in
-    let ntot' := ((Nat.iter (n + sum_crash_steps ns) step_count_next ncurr)) in
-    £ ntot -∗
-    (||={⊤|⊤, ∅|∅}=> ||▷=>^ntot ||={∅|∅, ⊤|⊤}=> (∃ e2 t2',
+  wptp s t1 -∗ NC 1-∗ step_fupdN_fresh ns HG (λ HG',
+    (|={⊤|⊤}⧗=>^n ||={⊤|⊤, ⊤|⊤}=> (∃ e2 t2',
     ⌜ t2 = e2 :: t2' ⌝ ∗
     state_interp σ2 (length t2') ∗
-    global_state_interp g2 ntot' mj D κs' ∗
+    global_state_interp g2 mj D κs' ∗
     from_option (Φr HG') True (to_val e2) ∗
     □ Φinv' HG' ∗
     ([∗ list] v ∈ omap to_val t2', fork_post v) ∗
     NC 1))).
 Proof.
-  revert HG e1 t1 κs κs' t2 σ1 g1 ncurr σ2 Φ.
-  induction ns as [|n' ns' IH] => HG e1 t1 κs κs' t2 σ1 g1 ncurr σ2 Φ.
+  revert HG e1 t1 κs κs' t2 σ1 g1 σ2 Φ.
+  induction ns as [|n' ns' IH] => HG e1 t1 κs κs' t2 σ1 g1 σ2 Φ.
   { rewrite app_nil_l.
     inversion 1.
     match goal with
@@ -154,56 +130,19 @@ Proof.
   rewrite {1}/step_fupdN_fresh -/step_fupdN_fresh.
   destruct ρ2 as (?&[σ2_pre_crash g2_pre_crash]).
   rewrite -assoc wpr_unfold /wpr_pre.
-  rewrite Nat.iter_succ.
-  iIntros "Hlc".
-  iPoseProof (@wptp_strong_crash_adequacy with "[$] [$] [$] [$] [$] [$]") as "H"; eauto.
-  iMod "H". iModIntro.
-  iApply (step_fupd2N_wand (steps_sum num_laters_per_step step_count_next ncurr (S n'))
-            with "H").
-  iIntros "H".
-  iMod "H".
-  iModIntro. iMod (fupd2_mask_subseteq ∅ ∅) as "Hclo"; [set_solver+..|].
-  iModIntro. iModIntro. iNext.
-  iMod ("Hclo") as "_".
-  iMod (fupd2_mask_subseteq ∅ ∅) as "Hclo"; [set_solver+..|].
-  iMod ("Hclo") as "_".
+  iPoseProof (@wptp_strong_crash_adequacy with "[$] [$] [$] [$] [$]") as "H"; eauto.
+  rewrite Nat.iter_succ_r.
+  iApply (physical_stepN_wand with "H"). iIntros ">H".
   iDestruct "H" as (e2 t2' ?) "(H&Hσ&Hg&HC)".
-  iMod ("H" with "[//] Hσ Hg") as "H".
-  iMod (fupd2_mask_subseteq ∅ ∅) as "Hclo"; [set_solver+..|]. do 2 iModIntro. iNext.
-  iModIntro.
-  iMod ("Hclo") as "_".
-  iModIntro.
+  iDestruct ("H" with "[//] Hσ Hg") as "H".
+  iApply (physical_step_subseteq ⊤ D); auto.
+  iApply (physical_step_wand with "H").
+  iDestruct 1 as (HG') "(HNC&Hσ&Hg&Hr)".
   destruct s0.
-  - iMod "H" as (HG') "(HNC&Hσ&Hg&Hr)".
-    iDestruct "Hr" as "(_&Hr)".
+  - iDestruct "Hr" as "(_&Hr)".
     simpl in *.
     iPoseProof (IH with "[Hσ] [Hg] Hr [] [] HNC") as "H"; eauto.
-    iExists _. iModIntro. simpl. eauto.
-    iApply (step_fupdN_fresh_wand with "H").
-    { auto. }
-    iIntros (HG'') "H Hlc".
-    iSpecialize ("H" with "[Hlc]").
-    { iExactEq "Hlc". f_equal.
-      rewrite {1}Nat.add_comm ?Nat.iter_add.
-      f_equal. rewrite -Nat.iter_succ -Nat.iter_succ_r //. }
-    iMod "H". iModIntro.
-    iEval rewrite -Nat.iter_succ Nat.iter_succ_r.
-    iApply step_fupd2N_le; last iApply (step_fupd2N_wand with "H").
-    { apply Nat.eq_le_incl. f_equal.
-      rewrite {1}Nat.add_comm ?Nat.iter_add.
-      f_equal. rewrite -Nat.iter_succ -Nat.iter_succ_r //. }
-    iIntros ">H".
-    rewrite {1}Nat.add_comm ?Nat.iter_add.
-    iDestruct "H" as (?? Heq) "(H1&Hg&?&?)".
-    iExists _, _. iFrame "∗".
-    iSplitL ""; first eauto.
-    iMod (global_state_interp_le with "Hg") as "$".
-    { apply Nat.eq_le_incl.
-      rewrite -?Nat.iter_succ_r -?Nat.iter_add Nat.add_assoc.
-      f_equal. lia. }
-    iModIntro; done.
-  - iMod "H" as (HG') "(HNC&Hσ&Hg&Hr)".
-    iExists HG'.
+  - iExists HG'.
     iAssert (□Φinv' HG')%I as "#Hinv'".
     { iDestruct "Hr" as "(Hr&_)".
       iApply "Hinv". eauto.
@@ -211,40 +150,27 @@ Proof.
     iDestruct "Hr" as "(_&Hr)".
     assert (ns' = []) as ->; first by (eapply nrsteps_normal_empty_prefix; eauto).
     iDestruct (wptp_recv_strong_normal_adequacy (HG:=HG') with "[Hσ] [Hg] [Hr] [] HNC") as "H"; eauto.
-    iModIntro.
-    iIntros "Hlc".
-    iClear "HC". simpl.
-    iSpecialize ("H" with "[Hlc]").
-    { iExactEq "Hlc". f_equal. rewrite Nat.add_0_r. done. }
-    iApply (step_fupd2N_inner_wand with "H"); try set_solver+.
-    { rewrite Nat.add_0_r. auto. }
-    iIntros "H".
-    iFrame "Hinv'". rewrite Nat.add_0_r.
-    rewrite -Nat.iter_succ Nat.iter_succ_r.
-    rewrite Nat.iter_add Nat.iter_succ_r.
-    eauto.
+    simpl.
+    iApply (physical_stepN_wand with "H").
+    iIntros ">H !>".
+    iFrame "# ∗".
 Qed.
 
 (* unfortunately this duplicates the large induction above.
 There is probably some way to factor this... *)
-Lemma wptp_recv_crash_progress {CS Φ Φinv Φinv' Φr κs' HG} ncurr mj D ns n r1 e1 t1 κs t2 σ1 g1 σ2 g2 ee2 :
+Lemma wptp_recv_crash_progress {CS Φ Φinv Φinv' Φr κs' HG} mj D ns n r1 e1 t1 κs t2 σ1 g1 σ2 g2 ee2 :
   nrsteps (CS := CS) r1 (ns ++ [n]) (e1 :: t1, (σ1,g1)) κs (t2, (σ2,g2)) Crashed →
   ee2 ∈ t2 →
   state_interp σ1 (length t1) -∗
-  global_state_interp g1 ncurr mj D (κs ++ κs') -∗
+  global_state_interp g1 mj D (κs ++ κs') -∗
   wpr CS NotStuck HG ⊤ e1 r1 Φ Φinv Φr -∗
   □ (∀ HG', Φinv HG' -∗ □ Φinv' HG') -∗
-  wptp NotStuck t1 -∗ NC 1-∗ step_fupdN_fresh ncurr ns HG (λ HG',
-    let ntot := (steps_sum num_laters_per_step step_count_next
-                           (Nat.iter (sum_crash_steps ns) step_count_next ncurr )
-                           n)  in
-    let ntot' := ((Nat.iter (n + sum_crash_steps ns) step_count_next ncurr)) in
-    £ (ntot + num_laters_per_step ntot' + 1) -∗
-    (||={⊤|⊤, ∅|∅}=> ||▷=>^ntot ||={∅|∅, ∅|∅}=> ||▷=>^(num_laters_per_step ntot' + 1)
+  wptp NotStuck t1 -∗ NC 1-∗ step_fupdN_fresh ns HG (λ HG',
+    (|={⊤|⊤}⧗=>^n ||={⊤|⊤, ∅|∅}=>
     ⌜ not_stuck ee2 σ2 g2 ⌝)).
 Proof.
-  revert HG e1 t1 κs κs' t2 σ1 g1 ncurr σ2 Φ.
-  induction ns as [|n' ns' IH] => HG e1 t1 κs κs' t2 σ1 g1 ncurr σ2 Φ.
+  revert HG e1 t1 κs κs' t2 σ1 g1 σ2 Φ.
+  induction ns as [|n' ns' IH] => HG e1 t1 κs κs' t2 σ1 g1 σ2 Φ.
   { rewrite app_nil_l.
     inversion 1.
     match goal with
@@ -256,54 +182,19 @@ Proof.
   rewrite {1}/step_fupdN_fresh -/step_fupdN_fresh.
   destruct ρ2 as (?&[σ2_pre_crash g2_pre_crash]).
   rewrite -assoc wpr_unfold /wpr_pre.
-  rewrite Nat.iter_succ.
-  iIntros "Hlc".
-  iPoseProof (@wptp_strong_crash_adequacy with "[$] [$] [$] [$] [$] [$]") as "H"; eauto.
-  iMod "H". iModIntro.
-  iApply (step_fupd2N_wand (steps_sum num_laters_per_step step_count_next ncurr (S n'))
-            with "H").
-  iIntros "H".
-  iMod "H".
-  iModIntro. iMod (fupd2_mask_subseteq ∅ ∅) as "Hclo"; [set_solver+..|].
-  iModIntro. iModIntro. iNext.
-  iMod ("Hclo") as "_".
-  iMod (fupd2_mask_subseteq ∅ ∅) as "Hclo"; [set_solver+..|].
-  iMod ("Hclo") as "_".
+  iPoseProof (@wptp_strong_crash_adequacy with "[$] [$] [$] [$] [$]") as "H"; eauto.
+  rewrite Nat.iter_succ_r.
+  iApply (physical_stepN_wand with "H"). iIntros ">H".
   iDestruct "H" as (e2 t2' ?) "(H&Hσ&Hg&HC)".
-  iMod ("H" with "[//] Hσ Hg") as "H".
-  iMod (fupd2_mask_subseteq ∅ ∅) as "Hclo"; [set_solver+..|]. do 2 iModIntro. iNext.
-  iModIntro.
-  iMod ("Hclo") as "_".
-  iModIntro.
+  iDestruct ("H" with "[//] Hσ Hg") as "H".
+  iApply (physical_step_subseteq ⊤ D); auto.
+  iApply (physical_step_wand with "H").
+  iDestruct 1 as (HG') "(HNC&Hσ&Hg&Hr)".
   destruct s0.
-  - iMod "H" as (HG') "(HNC&Hσ&Hg&Hr)".
-    iDestruct "Hr" as "(_&Hr)".
+  - iDestruct "Hr" as "(_&Hr)".
     simpl in *.
     iPoseProof (IH with "[Hσ] [Hg] Hr [] [] HNC") as "H"; eauto.
-    iExists _. iModIntro. simpl. eauto.
-    iApply (step_fupdN_fresh_wand with "H").
-    { auto. }
-    iIntros (HG'') "H Hlc".
-    iSpecialize ("H" with "[Hlc]").
-    { iExactEq "Hlc". f_equal. f_equal. f_equal.
-      - rewrite {1}Nat.add_comm ?Nat.iter_add.
-        f_equal. rewrite -Nat.iter_succ -Nat.iter_succ_r //.
-      - rewrite -?Nat.iter_succ_r -?Nat.iter_add.
-        f_equal. f_equal. lia. }
-    iMod "H". iModIntro.
-    iEval rewrite -Nat.iter_succ Nat.iter_succ_r.
-    iApply step_fupd2N_le; last iApply (step_fupd2N_wand with "H").
-    { apply Nat.eq_le_incl. f_equal.
-      rewrite {1}Nat.add_comm ?Nat.iter_add.
-      f_equal. rewrite -Nat.iter_succ -Nat.iter_succ_r //. }
-    iIntros ">H".
-    rewrite {1}[n + _]Nat.add_comm ?Nat.iter_add.
-    iModIntro. iApply (step_fupd2N_le with "H"); auto.
-    apply Nat.eq_le_incl. f_equal.
-    rewrite -?Nat.iter_succ_r -?Nat.iter_add Nat.add_assoc.
-    f_equal. lia.
-  - iMod "H" as (HG') "(HNC&Hσ&Hg&Hr)".
-    iExists HG'.
+  - iExists HG'.
     iAssert (□Φinv' HG')%I as "#Hinv'".
     { iDestruct "Hr" as "(Hr&_)".
       iApply "Hinv". eauto.
@@ -311,47 +202,21 @@ Proof.
     iDestruct "Hr" as "(_&Hr)".
     iDestruct (wptp_recv_normal_progress (HG:=HG') with "[Hσ] [Hg] [Hr] [] HNC") as "H"; eauto.
     iApply (step_fupdN_fresh_wand with "H").
-    { simpl. lia. }
-    iModIntro.
     iIntros (HG'') "H".
-    iDestruct "H" as (->) "H".
-    rewrite steps_sum_S_r.
-    iClear "HC". simpl.
-    assert (ns' = []) as ->; first by (eapply nrsteps_normal_empty_prefix; eauto).
-    iIntros "Hlc".
-    iSpecialize ("H" with "[Hlc]").
-    { simpl. rewrite Nat.add_0_r. iExactEq "Hlc". f_equal.
-      rewrite -assoc. f_equal.
-      rewrite ![_ + 1]comm. f_equal.
-      rewrite -Nat.iter_succ Nat.iter_succ_r.
-      rewrite Nat.iter_add Nat.iter_succ_r. done. }
-    simpl. iMod "H".
-    iApply (step_fupd2N_inner_wand with "H"); try set_solver+.
-    { rewrite Nat.add_0_r. auto. }
-    iIntros "H".
-    rewrite Nat.add_0_r.
-    rewrite -Nat.iter_succ Nat.iter_succ_r.
-    rewrite ![_ + 1]comm. simpl.
-    rewrite Nat.iter_add Nat.iter_succ_r.
-    eauto.
+    by iDestruct "H" as (->) "H".
 Qed.
 
-Lemma wptp_recv_strong_adequacy {CS Φ Φinv Φinv' Φr κs' s HG} ns mj D n r1 e1 t1 κs t2 σ1 g1 ncurr σ2 g2 stat :
+Lemma wptp_recv_strong_adequacy {CS Φ Φinv Φinv' Φr κs' s HG} ns mj D n r1 e1 t1 κs t2 σ1 g1 σ2 g2 stat :
   nrsteps (CS := CS) r1 (ns ++ [n]) (e1 :: t1, (σ1,g1)) κs (t2, (σ2,g2)) stat →
   state_interp σ1 (length t1) -∗
-  global_state_interp g1 ncurr mj D (κs ++ κs') -∗
+  global_state_interp g1 mj D (κs ++ κs') -∗
   wpr CS s HG ⊤ e1 r1 Φ Φinv Φr -∗
   □ (∀ HG', Φinv HG' -∗ □ Φinv' HG') -∗
-  wptp s t1 -∗ NC 1-∗ step_fupdN_fresh ncurr ns HG (λ HG',
-    let ntot := (steps_sum num_laters_per_step step_count_next
-                           (Nat.iter (sum_crash_steps ns) step_count_next ncurr )
-                           n)  in
-    let ntot' := ((Nat.iter (n + sum_crash_steps ns) step_count_next ncurr)) in
-    £ ntot -∗
-    (||={⊤|⊤, ∅|∅}=> ||▷=>^ntot ||={∅|∅, ⊤|⊤}=> (∃ e2 t2',
+  wptp s t1 -∗ NC 1-∗ step_fupdN_fresh ns HG (λ HG',
+    (|={⊤|⊤}⧗=>^n ||={⊤|⊤, ⊤|⊤}=> (∃ e2 t2',
     ⌜ t2 = e2 :: t2' ⌝ ∗
     state_interp σ2 (length t2') ∗
-    global_state_interp g2 ntot' mj D κs' ∗
+    global_state_interp g2 mj D κs' ∗
     (match stat with
      | Normal => ⌜ HG' = HG ⌝ ∗ from_option Φ True (to_val e2)
      | Crashed => from_option (Φr HG') True (to_val e2) ∗ □ Φinv' HG'
@@ -362,56 +227,41 @@ Proof.
   intros. destruct stat.
   - iIntros. iDestruct (wptp_recv_strong_crash_adequacy with "[$] [$] [$] [$] [$] [$]") as "H"; eauto.
     iApply (step_fupdN_fresh_wand with "H"); first auto.
-    iIntros (?) "H Hlc". iSpecialize ("H" with "Hlc").
-    iApply (step_fupd2N_wand with "H"); auto.
-    iIntros "H".
-    iMod "H" as (???) "(?&H&?&?&?)". iExists _, _.
+    iIntros (?) "H".
+    iApply (physical_stepN_wand with "H").
+    iMod 1 as (???) "(?&H&?&?&?)". iExists _, _.
     repeat (iSplitL ""; try iFrame; eauto).
   - iIntros.
     assert (ns = []) as ->; first by (eapply nrsteps_normal_empty_prefix; eauto).
     iDestruct (wptp_recv_strong_normal_adequacy with "[$] [$] [$] [$] [$]") as "H"; eauto.
-    iIntros "Hlc".
-    simpl. rewrite Nat.add_0_r. iSpecialize ("H" with "Hlc").
-    iMod "H". iModIntro.
-    iApply (step_fupd2N_wand with "H"); auto.
-    iIntros "H".
-    iMod "H" as (???) "(?&H&?&?&?)". iExists _, _.
+    iApply (physical_stepN_wand with "H").
+    iMod 1 as (???) "(?&H&?&?&?)". iExists _, _.
     iSplitL ""; first eauto. iFrame. eauto.
 Qed.
 
-Lemma wptp_recv_progress {CS Φ Φinv Φinv' Φr κs' HG} ns mj D n r1 e1 t1 κs t2 σ1 g1 ncurr σ2 g2 stat e2 :
+Lemma wptp_recv_progress {CS Φ Φinv Φinv' Φr κs' HG} ns mj D n r1 e1 t1 κs t2 σ1 g1 σ2 g2 stat e2 :
   nrsteps (CS := CS) r1 (ns ++ [n]) (e1 :: t1, (σ1,g1)) κs (t2, (σ2,g2)) stat →
   e2 ∈ t2 →
   state_interp σ1 (length t1) -∗
-  global_state_interp g1 ncurr mj D (κs ++ κs') -∗
+  global_state_interp g1 mj D (κs ++ κs') -∗
   wpr CS NotStuck HG ⊤ e1 r1 Φ Φinv Φr -∗
   □ (∀ HG', Φinv HG' -∗ □ Φinv' HG') -∗
-  wptp NotStuck t1 -∗ NC 1-∗ step_fupdN_fresh ncurr ns HG (λ HG',
-    let ntot := (steps_sum num_laters_per_step step_count_next
-                           (Nat.iter (sum_crash_steps ns) step_count_next ncurr )
-                           n)  in
-    let ntot' := ((Nat.iter (n + sum_crash_steps ns) step_count_next ncurr)) in
-    £ (ntot + num_laters_per_step ntot' + 1) -∗
-    (||={⊤|⊤, ∅|∅}=> ||▷=>^ntot ||={∅|∅, ∅|∅}=> ||▷=>^(num_laters_per_step ntot' + 1)
+  wptp NotStuck t1 -∗ NC 1-∗ step_fupdN_fresh ns HG (λ HG',
+    (|={⊤|⊤}⧗=>^n ||={⊤|⊤ , ∅|∅}=> 
     ⌜ not_stuck e2 σ2 g2 ⌝)).
 Proof.
   intros. destruct stat.
   - iIntros. iDestruct (wptp_recv_crash_progress with "[$] [$] [$] [$] [$] [$]") as "H"; eauto.
   - iIntros. iDestruct (wptp_recv_normal_progress with "[$] [$] [$] [$] [$]") as "H"; eauto.
     iApply (step_fupdN_fresh_wand with "H"); first auto.
-    iIntros (?) "H Hlc".
-    iDestruct "H" as (->) "H".
+    iIntros (?).
+    iDestruct 1 as (->) "H".
     assert (ns = []) as ->; first by (eapply nrsteps_normal_empty_prefix; eauto).
-    rewrite steps_sum_S_r.
-    simpl. rewrite Nat.add_0_r.
-    iMod ("H" with "[Hlc]") as "H".
-    { iExactEq "Hlc". f_equal. lia. } 
-    iModIntro.
-    iApply (step_fupd2N_wand with "H"); auto.
+    done.
 Qed.
 
 End recovery_adequacy.
-
+(* 
 Fixpoint fresh_later_count f g ncurr (ns: list nat) :=
   match ns with
   | [] => 0
@@ -425,60 +275,44 @@ Proof. simpl. lia. Qed.
 Lemma fresh_later_count_cons f g ncurr n (ns': list nat) :
   fresh_later_count f g ncurr (n::ns') = crash_adequacy.steps_sum f g ncurr (S n) + 3
                  + fresh_later_count f g (Nat.iter (S n) g ncurr) ns'.
-Proof. simpl. lia. Qed.
+Proof. simpl. lia. Qed. *)
 
-Lemma step_fupdN_fresh_rearrange {Λ Σ} `{!irisGS Λ Σ} {HG : generationGS Λ Σ} φ ns ncurr k k2:
-  (|={⊤}=> step_fupdN_fresh ncurr ns _
-                  (λ _, £ (k + k2) -∗ ||={⊤|⊤,∅|∅}=> ||▷=>^k ||={∅|∅,∅|∅}=> ||▷=>^k2 ⌜φ⌝)) -∗
-  £ (fresh_later_count num_laters_per_step step_count_next ncurr ns + k + k2) -∗
-  ||={⊤|⊤,∅|∅}=> ||▷=>^(fresh_later_count num_laters_per_step step_count_next ncurr ns + S k + k2) ⌜φ⌝.
+Lemma step_fupdN_fresh_rearrange {Λ Σ} `{!irisGS Λ Σ} {HG : generationGS Λ Σ} φ ns k:
+  (|={⊤}=> step_fupdN_fresh ns _
+                  (λ _, |={⊤|⊤}⧗=>^k ||={⊤|⊤, ∅|∅}=> ⌜φ⌝)) -∗
+    ||={⊤|⊤, ⊤|⊤}=> |={⊤|⊤}⧗=>^((sum_list $ fmap S $ ns) + k) ||={⊤|⊤, ∅|∅}=> ⌜φ⌝.
 Proof.
-  iIntros "H Hlc".
-  iInduction ns as [| n' ns] "IH" forall (HG ncurr).
+  iIntros "H".
+  iInduction ns as [| n' ns] "IH" forall (HG).
   - rewrite /step_fupdN_fresh.
-    iMod "H". iMod ("H" with "Hlc") as "H". iModIntro.
-    rewrite fresh_later_count_nil.
-    replace (0 + S k) with (k + 1) by lia.
-    rewrite -!assoc -step_fupd2N_add.
-    iApply (step_fupd2N_wand with "H"). iIntros "H".
-    rewrite -step_fupd2N_add.
-    iMod "H". iApply (fupd2_mask_intro); [done..|]. iIntros "_".
-    done.
+    simpl. by iMod "H".
   - iMod NC_alloc as (Hc') "HNC".
     rewrite /step_fupdN_fresh -/step_fupdN_fresh.
-    iMod "H".
-    rewrite fresh_later_count_cons.
-    iEval (rewrite !lc_split -assoc) in "Hlc".
-    iDestruct "Hlc" as "[[[Hlc1 _] Hlc2] Hlck]".
-    iMod ("H" with "Hlc1") as "H". iModIntro.
-    rewrite -!assoc -step_fupd2N_add.
-    iApply (step_fupd2N_wand with "H"). iIntros "H".
-    iApply step_fupd2_fupd2N; first lia.
-    do 2 iMod "H". iModIntro.
-    rewrite -step_fupd2N_add. replace 3 with (2+1) by lia.
-    rewrite -step_fupd2N_add.
-    iApply (step_fupd2N_wand with "H"). iIntros "H".
-    iMod "H".
-    iMod "H" as (HG') "H".
-    iMod ("IH" $! HG' with "H [Hlc2 Hlck]") as "H".
-    { iEval rewrite !lc_split. by iFrame. }
-    do 3 iModIntro. rewrite assoc. done.
+    iMod "H". simpl. iModIntro. iEval (rewrite -Nat.add_assoc Nat.iter_add).
+    rewrite -!Nat.iter_succ.
+    iApply (physical_stepN_S_fupd).
+    iApply (physical_stepN_wand with "H").
+    iDestruct 1 as (HG') "H".
+    iApply ("IH" $! HG' with "H").
 Qed.
 
-Lemma step_fupdN_fresh_soundness {Λ Σ} `{!invGpreS Σ} `{!crashGpreS Σ} (φ : Prop) ns ncurr k k2 f g:
-  (∀ (Hi: invGS Σ) (Hc: crashGS Σ), NC 1 ={⊤}=∗
-    ∃ (HI: irisGS Λ Σ) (HG:generationGS Λ Σ) (Hpf1: iris_invGS = Hi)
-     (Hpf2: num_laters_per_step = f) (Hpf2: step_count_next = g) (Hpf4: iris_crashGS = Hc),
-      (|={⊤}=> step_fupdN_fresh ncurr ns HG (λ _,
-       £ (k + k2) -∗ ||={⊤|⊤,∅|∅}=> ||▷=>^k ||={∅|∅,∅|∅}=> ||▷=>^k2 ⌜φ⌝))%I) →
+Axiom functional_extensionality: forall {A B} (f g:A->B) , (forall x, f x = g x) -> f = g.
+
+Lemma step_fupdN_fresh_soundness {Λ Σ} `{!invGpreS Σ} `{!trGpreS Σ} `{Htrgen : !tr_generation} `{!crashGpreS Σ} (φ : Prop) ns k n:
+  (∀ (Hi: invGS Σ) (Htr : trGS Σ) (Hc: crashGS Σ), ⧗ n ∗ £ n -∗ NC 1 ={⊤}=∗
+    ∃ (HI: irisGS Λ Σ) (HG:generationGS Λ Σ) (Hpf1: iris_invGS = Hi) (Hpf2: iris_trGS = Htr) (Hpf3: iris_trGen = Htrgen) (Hpf4: iris_crashGS = Hc),
+      (|={⊤}=> step_fupdN_fresh ns HG (λ _,
+        |={⊤|⊤}⧗=>^k ||={⊤|⊤, ∅|∅}=>
+        ⌜φ⌝))%I) →
   φ.
 Proof.
   intros Hiter.
-  eapply (step_fupd2N_soundness (fresh_later_count f g ncurr ns + S k + k2) (fresh_later_count f g ncurr ns + k + k2)).
-  iIntros (Hinv) "Hlc".
+  eapply pure_soundness.
+  eapply (physical_stepN_soundness _ n (sum_list (S <$> ns) + k)) => Hinv Htr.
+  iIntros "H⧗£".
   iMod NC_alloc as (Hc) "HNC".
-  iMod (Hiter Hinv Hc with "HNC") as (Hiris Hgen <- <- <- <-) "H".
-  iApply (step_fupdN_fresh_rearrange with "H Hlc").
+  iMod (Hiter Hinv Htr Hc with "H⧗£ HNC") as (Hiris Hgen <- <- <- <-) "H".
+  iApply (step_fupdN_fresh_rearrange φ ns k with "H").
 Qed.
 
 Record recv_adequate {Λ CS} (s : stuckness) (e1 r1: expr Λ) (σ1 : state Λ) (g1 : global_state Λ)
@@ -514,18 +348,18 @@ Proof.
   - constructor; naive_solver.
 Qed.
 
-Corollary wp_recv_adequacy_inv Σ Λ CS `{!invGpreS Σ} `{!crashGpreS Σ} nsinit s e r σ g φ φr φinv f1 f2:
-  (∀ `(Hinv : !invGS Σ) `(Hc: !crashGS Σ) κs,
-     ⊢ |={⊤}=> ∃
+Corollary wp_recv_adequacy_inv Σ Λ CS `{!invGpreS Σ} `{!trGpreS Σ} `{Htrgen : !tr_generation} `{!crashGpreS Σ} s e r σ g φ φr φinv ntr:
+  (∀ `(Hinv : !invGS Σ) `(Htr : !trGS Σ) `(Hc: !crashGS Σ) κs,
+     ⧗ ntr ∗ £ ntr ⊢ |={⊤}=> ∃
          (stateI : state Λ → nat → iProp Σ) (* for the initial generation *)
-         (global_stateI : global_state Λ → nat → fracR → coPset → list (observation Λ) → iProp Σ)
-         (fork_post : val Λ → iProp Σ) Hpf1a Hpf1b
+         (global_stateI : global_state Λ → fracR → coPset → list (observation Λ) → iProp Σ)
+         (fork_post : val Λ → iProp Σ)
          Φinv,
-        let HI := IrisGS Λ Σ Hinv (global_stateI) (fork_post) f1 f2 Hpf1a Hpf1b in
+        let HI := IrisGS Λ Σ Hinv Htr Htrgen (global_stateI) (fork_post) in
         let HG := GenerationGS Λ Σ Hc stateI in
        □ (∀ σ nt, stateI σ nt -∗ |NC={⊤, ∅}=> ⌜ φinv σ ⌝) ∗ (* φinv for initial gen. *)
        □ (∀ HG, Φinv Hinv HG -∗ □ ∀ σ nt, state_interp σ nt -∗ |@NC={iris_crashGS, ⊤, ∅}=> ⌜ φinv σ ⌝) ∗ (* φinv for later generations *)
-       stateI σ 0 ∗ global_stateI g nsinit 1%Qp ∅ κs ∗
+       stateI σ 0 ∗ global_stateI g 1%Qp ∅ κs ∗
        wpr CS s HG ⊤ e r (λ v, ⌜φ v⌝) (Φinv Hinv) (λ _ v, ⌜φr v⌝)) →
   recv_adequate (CS := CS) s e r σ g (λ v _ _, φ v) (λ v _ _, φr v) (λ σ _, φinv σ).
 Proof.
@@ -536,15 +370,12 @@ Proof.
      probably we can somehow avoid all this code duplication... *)
   split; last first.
   { destruct (nrsteps_snoc _ _ _ _ _ _ H) as (ns'&n'&->).
-  eapply (step_fupdN_fresh_soundness _ ns' nsinit
-              (crash_adequacy.steps_sum f1 f2 (Nat.iter (sum_crash_steps ns') f2 nsinit) n')
-               (S (S  (f1 (Nat.iter (n' + sum_crash_steps ns') f2 nsinit)))))
-         => Hinv Hc.
-  iIntros "HNC".
-  iMod (Hwp Hinv Hc κs) as (stateI global_stateI fork_post Hpf1a Hpf1b) "H".
-  iDestruct "H" as (Φinv) "(#Hinv1&#Hinv2&Hσ&Hg&H)".
+  eapply (step_fupdN_fresh_soundness _ ns')
+         => Hinv Htr Hc.
+  iIntros "H⧗£ HNC".
+  iMod (Hwp Hinv Htr Hc κs with "H⧗£") as (stateI global_stateI fork_post Φinv) "(#Hinv1&#Hinv2&Hσ&Hg&H)".
   iModIntro.
-  set (HI := IrisGS Λ Σ Hinv (global_stateI) (fork_post) f1 f2 Hpf1a Hpf1b).
+  set (HI := IrisGS Λ Σ Hinv Htr _ (global_stateI) (fork_post)).
   set (HG := GenerationGS Λ Σ Hc stateI).
   iExists HI, HG.
   iDestruct (wptp_recv_strong_adequacy
@@ -554,41 +385,33 @@ Proof.
   do 4 iExists eq_refl.
   iModIntro.
   iApply (step_fupdN_fresh_wand with "H").
-  { auto. }
-  iIntros (HG') "H [Hlc1 Hlc2]".
-  iMod ("H" with "Hlc1") as "H".
-  iApply (step_fupd2N_wand with "H"); auto.
-  iModIntro. iIntros "H".
-  iMod "H" as (v2 ??) "(Hσ&Hg&Hv&Hfpost&HNC)".
+  iIntros (HG') "H".
+  iApply (physical_stepN_wand with "H").
+  iMod 1 as (v2 ??) "(Hσ&Hg&Hv&Hfpost&HNC)".
   destruct stat.
   - iDestruct "Hv" as "(Hv&#Hinv)".
     rewrite ?ncfupd_eq /ncfupd_def.
-    iMod ("Hinv" with "[$] [$]") as "(Hp&HNC)".
-    iApply fupd2_mask_intro; [done..|]. iIntros "_".
-    iApply step_fupd2N_later.
-    repeat iModIntro. iSplit; last done.
-    iIntros (v2' ? Heq). subst. inversion Heq; subst.
+    iMod ("Hinv" with "[$] [$]") as "(%&HNC)".
+    iApply fupd2_mask_intro; [done..|]. iIntros.
+    iSplit; last done. iIntros (v2' ? Heq). subst. inversion Heq; subst.
     rewrite to_of_val. naive_solver.
   - iDestruct "Hv" as "(->&Hv)".
     rewrite ?ncfupd_eq /ncfupd_def.
     iMod ("Hinv1" with "[$] [$]") as "(Hp&HNC)".
     iApply fupd2_mask_intro; [done..|]. iIntros "_".
-    iApply step_fupd2N_later.
-    repeat iModIntro. iSplit; last done.
+    iSplit; last done.
     iIntros (v2' ? Heq). subst. inversion Heq; subst.
     rewrite to_of_val. naive_solver.
   }
   { intros e2 -> He2.
   destruct (nrsteps_snoc _ _ _ _ _ _ H) as (ns'&n'&->).
-  eapply (step_fupdN_fresh_soundness _ ns' nsinit
-              (crash_adequacy.steps_sum f1 f2 (Nat.iter (sum_crash_steps ns') f2 nsinit) n')
-                (f1 (Nat.iter (n' + sum_crash_steps ns') f2 nsinit) + 1))
-         => Hinv Hc.
-  iIntros "HNC".
-  iMod (Hwp Hinv Hc κs) as (stateI global_stateI fork_post Hpf1a Hpf1b) "H".
+  eapply (step_fupdN_fresh_soundness _ ns')
+         => Hinv Htr Hc.
+  iIntros "H⧗£ HNC".
+  iMod (Hwp Hinv Htr Hc κs with "H⧗£") as (stateI global_stateI fork_post) "H".
   iDestruct "H" as (Φinv) "(#Hinv1&#Hinv2&Hσ&Hg&H)".
   iModIntro.
-  set (HI := IrisGS Λ Σ Hinv (global_stateI) (fork_post) f1 f2 Hpf1a Hpf1b).
+  set (HI := IrisGS Λ Σ Hinv Htr _ (global_stateI) (fork_post)).
   set (HG := GenerationGS Λ Σ Hc stateI).
   iExists HI, HG.
   iDestruct (wptp_recv_progress
@@ -596,9 +419,7 @@ Proof.
                (κs' := []) (HG := HG) with "[Hσ] [Hg] [H] [] [] HNC") as "H"; [eauto..|].
   { rewrite app_nil_r. eauto. }
   do 4 iExists eq_refl. iModIntro.
-  iApply (step_fupdN_fresh_wand with "H"); first done.
-  iIntros (?). iIntros "H Hlc".
-  iApply "H". iExactEq "Hlc". f_equiv; first done.
-  rewrite assoc. f_equiv. done.
+  iApply (step_fupdN_fresh_wand with "H").
+  iIntros (?) "$".
  }
 Qed.
